# **Survival Models**

Survival Models are probability distributions that measure the **time to failure** of an entity, or phrased another way, the **future lifetime** of an entity. In an Actuarial context, it measures the **time to death** of a person.

Since survival models measure *time*, they are denoted by the **continuous random variable** $T_i$, where the subscript represents the **age** of the person being studied.

## **Newborn Lifetime**

The base survival model measures the future lifetime of a newborn (**aged 0**), denoted by the random variable $T_0$.

The **CDF** thus represents the probability that the newborn **dies before age $t$**:

$$
    F_0(t) = P(T_0 \le t)
$$

The **Survival Function** is the **complement of the CDF** and is the probability that the newborn **survives till a certain age $t$**. From a different perspective, it can also be seen as the probability of the newborn **dying AFTER age $t$**:

$$
\begin{aligned}
    S_0(t)
    &= P(T_0 \ge t) \\
    &= 1 - P(T_0 \le t) \\
    &= 1 - F_0(t)
\end{aligned}
$$

Note that all humans will **inevitably die**:

$$
\begin{aligned}
    \lim_{t \to \infty} S_0 (t) = 0 \iff \lim_{t \to \infty} F_0 (t) = 1
\end{aligned}
$$

## **Continuous Lifetime**

The above can be **generalized** for a person aged $x$, denoted by $T_x$. However, the intepretation of the two functions changes slightly.

The CDF instead represents the probability that the person **dies within $t$ years** from age $x$:

$$
\begin{aligned}
    F_x(t) &= P(T_x \le t) \\
    T_x &= 1, 2, \dots
\end{aligned}
$$

It can also be written **in terms of the newborn lifetime**. The key is to understand that the newborn is **assumed to survive till age $x$** and then die within the next $t$ years:

$$
\begin{aligned}
    P(T_x \le t)
    &= P(T_0 \le x + t | T_0 > x) \\
    &= \frac{P(x < T_0 < x +t)}{P(T_0 > x)} \\
    &= \frac{P(T_0 < x +t)-P(T_0 < x)}{P(T_0 > x)} \\
    &= \frac{F_0(x+t) - F_0(x)}{S_0(x)}
\end{aligned}
$$

<!-- Self Made -->
![CDF Illustration](Assets/1.%20Survival%20Models.md/CDF%20Illustration.png){.center}

Conversely, the survival function is the probability that the person **survives another $t$ years** or **dies AFTER $t$ years**:

$$
    S_x(t) = P(T_x \ge t)
$$

It can also be written **in terms of the newborn lifetime** following the same logic as above. The newborn is **assumed to survive till age $x$** and then survive another $t$ years:

$$
\begin{aligned}
    P(T_x \ge t)
    &= P(T_0 \ge x + t | T_0 > x) \\
    &= \frac{P(T_0 > x + t)}{P(T_0 > x)} \\
    &= \frac{S_0(x+t)}{S_0(x)}
\end{aligned}
$$

> Note that since the surviving till age $x$ is a **subset** of surviving till age $x+t$, the numerator can be simplified to just surviving till $x+t$.

<!-- Self Made -->
![Survival Function Illustration](Assets/1.%20Survival%20Models.md/Survival%20Function%20Illustration.png){.center}

Note the survival function can thus be re-written as the following:

$$
\begin{aligned}
    S_x(t) &= \frac{S_0(x+t)}{S_0(x)} \\
    S_0(x+t) &= S_0(x)S_x(t) \\
\end{aligned}
$$

The probability of the survival of a newborn till age $x+t$ is the product of:

1. The probability of survival of a newborn till age $x$
2. Given that the newborn survived till age $x$, that they will survive another $t$ years

This can be **generalized** for people of any age to obtain:

$$
    S_x(t+u) = S_x(t) S_{x+t}(u)
$$

> It is important to remember to "update" the starting age of the second term to the "new age".

The *opposite* of the above is when an individual surives another $t$ years and then **dies within the following $u$ years**. This is known as the probability of **Deferred Death**:

$$
\begin{aligned}
    P(t < T_x < t+u)
    &= P(T_x < t+u) - P(T_x < t) \\
    &= F_x(t+u) - F_x(t) \\
    &= 1 - S_x(t+u) - (1 - S_x(t)) \\
    &= 1 - S_x(t)S_{x+t}(u) - 1 + S_x(t) \\
    &= S_x(t) - S_x(t)S_{x+t}(u) \\
    &= S_x(t)(1-S_{x+t}(u)) \\
    &= S_x(t)F_{x+t}(u)
\end{aligned}
$$

<!-- Self Made -->
![Deferred Death](Assets/1.%20Survival%20Models.md/Deferred%20Death%20Illustration.png){.center}

### **Probability Tree Perspective**

Since the probabilites of death and survival are conditional on the age of the individual, they can be better expressed in the form of a probability tree:

<!-- Self Made -->
![Probability Tree](Assets/1.%20Survival%20Models.md/Probability%20Tree.png)

Thus, it can be shown through *recursion* that the probability of surviving $t$ years is equal to the **sum of the probabilities of deferred deaths** for every year after:

$$
\begin{aligned}
    S_x(1)
    &= S_x(1)F_{x+1}(1) + S_x(1)S_{x+1}(1) \\
    &= S_x(1)F_{x+1}(1) + S_x(1) [S_{x+1}(1)F_{x+2}(1) + S_{x+1}(1)S_{x+2}(1)] \\
    &= S_x(1)F_{x+1}(1) + S_x(1) S_{x+1}(1)F_{x+2}(1) + S_x(1) S_{x+1}(1)S_{x+2}(1) \\
    &= S_x(1)F_{x+1}(1) + S_x(2)F_{x+2}(1) + S_x(2)S_{x+2}(1) \\
    &= S_x(1)F_{x+1}(1) + S_x(2)F_{x+2}(1) + \dots \\
    \\
    \therefore S_x(t) &= \sum S_x(t)F{x+t}(1)
\end{aligned}
$$

Recall that the probability of surviving till a certain age is simply the probability that the individual will die sometime *after* that age. The above expression solidifies this, where the RHS is the **probability of dying in every possible age after**.

### **Force of Mortality**

The **Force of Mortality** is the probability of dying *instantly*; in an **infinitely small unit of time** (normalized by unit time):

$$
\begin{aligned}
    \mu_x
    &= \lim_{h \to 0} \frac{P(T_x < h)}{h} \\
    &= \lim_{h \to 0} \frac{1 - S_x(h)}{h} \\
    &= \lim_{h \to 0} \frac{1 - (\frac{S_0(x+h)}{S_0(x)})}{h} \\
    &= \lim_{h \to 0} \frac{S_0(x) - S_0(x+h)}{S_0(x)h} \\
    &= \frac{1}{S_0(x)} \lim_{h \to 0} \frac{S_0(x) - S_0(x+h)}{h} \\
    &= - \frac{1}{S_0(x)} \lim_{h \to 0} \frac{S_0(x+h) - S_0(x)}{h} \\
    &= - \frac{1}{S_0(x)} S'_0(x) \\
    &= - \frac{S'_0(x)}{S_0(x)}
\end{aligned}
$$

Since $S_0(x)$ is the complement of $F_0(x)$, the derivative of the survival function can be written in terms of the PDF of the future lifetime:

$$
\begin{aligned}
    f_0(x)
    &= \frac{d}{dx} F_0(x) \\
    &= \frac{d}{dx} (1-S_0(x)) \\
    &= -S'_0(x)
\end{aligned}
$$

The force of mortality can be rewritten as the following:

$$
    \mu_x = \frac{f_0(x)}{S_0(x)}
$$

Thus, the force of mortality can also be intepreted as the **CONDITIONAL probability distribution** of death for a person aged $x$, *assuming* that the person survives till age $x$.

> $f_0(x)$ is UNCONDITIONAL distribution of the future lifetime as it does not assume the individual lives to any age.

#### **Alternative Death Function**

More generally, the force of mortality can be rewritten as:

$$
\begin{aligned}
    \mu_x &= \frac{f_0(x)}{S_0(x)} \\
    \mu_{x+t} &= \frac{f_x(t)}{S_x(t)} \\
    f_x(t) &= S_x(t)\mu_{x+t} \\
    F_x(t) &= \int_0^t S_x(t)\mu_{x+t}
\end{aligned}
$$

The probability of death in an interval is the SUM of the product of the probability of surviving till a given age and then dying in an infinitely small time afterwards. The sum of all the infinitely small time periods is equal to the given time interval.

Following this definition, for **extremely small time intervals**, the force of mortality can be used to *approximate* the probability of death in that interval:

$$
    P(T_x < h) \approx h * \mu_{x}
$$

#### **Alternative Survival Function**

More generally, the force of mortality can be rewritten as:

$$
\begin{aligned}
    \mu_{x} &= - \frac{S'_0(x)}{S_0(x)} \\
    \mu_{x + t} &= \frac{-S'_x(t)}{S_x(t)} \\
    \mu_{x + t} &= - \frac{d}{dt} (\ln S_x(t)) \\
    \ln S_x(t) &= - \int_{0}^{t} \mu_{x + t} \\
    S_x(t) &= e ^ {- \int_{0}^{t} \mu_{x + t}} \\
\end{aligned}
$$

> Note that most expressions give $\mu_x$, but it is $\mu_{x+t}$ that is usually of interest - simply adjust the parameters accordingly.

Thus, if $\mu_x$ is known for all ages, then the survival probabilites for any age can be calculated from it. In other words, the **distribution of $T_x$ can be determined from the force of mortality**.

### **Actuarial Notation**

Given how often these expressions are used, they are often abbreviated using the **International Actuarial Notation**:

$$
\begin{aligned}
    {}_{t}p_{x} &= S_x(t) \\
    {}_{t}q_{x} &= F_x(t) \\
    {}_{t}q_{x} + {}_{t}p_{x} &= 1
\end{aligned}
$$

> If $t=1$, it is omitted; EG. ${}_{1}q_{x} = q_{x}$.

Deferred Deaths are expressed using the pipe symbol:

$$
\begin{aligned}
    {}_{t|u}q_{x}
    &= S_x(t)F_{x+t}(u) \\
    &= {}_{t}p_{x} * {}_{u}q_{x+t}
\end{aligned}
$$

> These notations are *typically* used when $t$ is an integer, but not necessarily so, as will be seen in the next section.

### **Continuous Expectation**

The **Expectation** of the distribution of future lifetime is the **Life Expectancy** of the individual. It is commonly calculated for newborns as a measure of the general health of the population.

In an insurance context, it is known as the **Complete Expectation of Life** and is denoted by $\mathring{e}_{x}$:

$$
\begin{aligned}
    E(T_x) &= \int_{0}^{\infty} t f_x(t) \\
    e_{x} &= \int_{0}^{\infty} t S_x(t)\mu_{x+t}
\end{aligned}
$$

Through integration by parts,

$$
\begin{aligned}
    \mathring{e}_{x}
    &= \left(\Bigl[-tS_x(t)\Bigr]_0^\infty + \int_0^\infty S_x(t)\right) \\
    &= \int_0^\infty {}_{t}p_x
\end{aligned}
$$

> Note that $[-t * S_x(t)]^{\infty}_0$ is 0 as the probability of living forever is 0.

If the future lifetime variable is artificially limited to $n$ years, then the expectation of the future lifetime is known as the **Term Expectation of Life**. It is similar denoted as $\mathring{e}_{x:\enclose{actuarial}{n}}$:

$$
\begin{aligned}
    E(min(T_x, n)) &= \int^{n}_0 {}_{t}p_x \\
    \mathring{e}_{x:\enclose{actuarial}{n}} &= \int^{n}_0 {}_{t}p_x
\end{aligned}
$$

Thus, the complete expectation can be **decomposed** into two components:

1. **Term Expectation** at the *current age* representing the "early" years
2. **Complete Expectation** at a *future age* represenging the "later" years

$$
    \mathring{e}_x = \mathring{e}_{x:n} + \mathring{e}_{x+n}
$$

However, the above makes an implicit assumption that the individual **will survive** the first n years. Thus, the second term needs to account for the probability of surviving another n years:

$$
    \mathring{e}_x = \mathring{e}_{x:n} + {}_{n}p_x \cdot \mathring{e}_{x+n}
$$

### **Continuous Variance**

The second moment can be calculated in a similar fashion through integration by parts:

$$
\begin{aligned}
    E(T^2_x)
    &= \int_{0}^{\infty} t^2 f_x(t) \\
    &= -\left(\Bigl[t^2 S_x(t)\Bigr]_0^\infty - \int_{0}^{\infty} 2tS_x(t) \right) \\
    &= 2 \int_{0}^{\infty} t \cdot {}_{t}p_x
\end{aligned}
$$

Thus, the **Variance** of the future lifetime about the Expectation is the following:

$$
\begin{aligned}
    Var(T_x)
    &= E(T^2_x) - [E(T_x)]^2 \\
    &= 2 \int_{0}^{\infty} t \cdot {}_{t}p_x - \left(\int_0^\infty {}_{t}p_x \right)^2
\end{aligned}
$$

## **Discrete Lifetime**

If only the **integer components** of the future lifetime are considered, then it becomes a discrete distribution known as the **Curtate Future Lifetime** of the person.

It is denoted by the random variable $K_x$, which is a truncated version of $T_x$. Formally, it is known as a **Floor Function**:

$$
\begin{aligned}
    K_x &= \lfloor T_x \rfloor \\
    K_x &= 0, 1, \dots
\end{aligned}
$$

It measures the number of **full years** that the individual is expected to live for. If $K_x = k$, then it means the individual will another $k$ full years but not live past $k+1$ years full years. In other words, they will die between **$k$ (inclusive) and $k+1$ (Exclusive) years**.

> Note that the distribution **starts from 0**. If $K_x = 0$, then they will not live another full year; they will die within the current year.

$$
\begin{aligned}
    P(K_x = k)
    &= P(x+k \le T_0 < x+k+1) \\
    &= P(k \le T_x < k+1) \\
    &= P(T_x < k+1) - P(T_x \le k) \\
    &= F_x(k+1) - F_x(k) \\
    &= S_x(k) - S_x(k+1) \\
    &= S_x(k) - S_x(k) * S_{x+k}(1) \\
    &= S_x(k) (1 - S_{x+k}(1)) \\
    &= S_x(k) F_{x+k}(1) \\
    &= {} {}_{k}p_{x} {}_{}q_{x + k} \\
    &= {}_{k|}q_{x}
\end{aligned}
$$

<!-- Self Made -->
![Curtate Death Illustration](Assets/1.%20Survival%20Models.md/Curtate%20Death%20Illustration.png){.center}

### **Discrete Expectation**

Similarly, the Expected Curtate Lifetime is the expectation of $K_x$:

$$
\begin{aligned}
    e_x
    &=(K_x) \\
    &= \sum_{k=0}^{\infty} k ({}_{k}p_{x} - {}_{k+1}p_{x}) \\
    &= 1 ({}_{1}p_{x} - {}_{2}p_{x}) + 2 ({}_{2}p_{x} - {}_{3}p_{x}) + 3 ({}_{3}p_{x} - {}_{4}p_{x}) + ... \\
    &= {}_{1}p_{x} - {}_{2}p_{x} + 2{}_{2}p_{x} - 2{}_{3}p_{x} + 3 {}_{3}p_{x} - 3 {}_{4}p_{x} \\
    &= {}_{1}p_{x} + 2{}_{2}p_{x} + 3 {}_{3}p_{x} + ... \\
    &= \sum_{k=1}^{\infty} {}_{k}p_{x}
\end{aligned}
$$

The expectation can also **recursively** calculated:

* If the individual dies within the year with probability $q_x$, then the future lifetime is 0
* If the individual survives the year with probability $p_x$, then the future lifetime is 1 (for surviving the current year) AND the expected lifetime past that

$$
\begin{aligned}
    e_x
    &=
    \begin{cases}
        0,& q_x \\
        1+e_{x+1},& p_x
    \end{cases} \\
    \\
    \therefore e_x &= p_x (1+e_{x+1})
\end{aligned}
$$

### **Discrete Variance**

The second moment can be calculated in a similar fashion:

$$
\begin{aligned}
    E(K^2_x)
    &= \sum_{k=0}^{\infty} k^2 ({}_{k}p_{x} - {}_{k+1}p_{x}) \\
    &= 1 ({}_{1}p_{x} - {}_{2}p_{x}) + 4 ({}_{2}p_{x} - {}_{3}p_{x}) + 9 ({}_{3}p_{x} - {}_{4}p_{x}) + ... \\
    &= {}_{1}p_{x} - {}_{2}p_{x} + 4{}_{2}p_{x} - 4{}_{3}p_{x} + 9 {}_{3}p_{x} - 9 {}_{4}p_{x} \\
    &= {}_{1}p_{x} + 3{}_{2}p_{x} + 5 {}_{3}p_{x} + ... \\
    &= \sum_{k=1}^{\infty} (2k-1) {}_{k}p_{x} \\
    &= \sum_{k=1}^{\infty} 2k{}_{k}p_{x} - {}_{k}p_{x} \\
    &= \sum_{k=1}^{\infty} 2k{}_{k}p_{x} - \sum_{k=1}^{\infty} {}_{k}p_{x} \\
    &= 2 \sum_{k=1}^{\infty} k{}_{k}p_{x} - e_x
\end{aligned}
$$

Thus, the variance can be calculated as:

$$
\begin{aligned}
    Var(K_x)
    &= E(K_x^2) - [E(K_x)]^2 \\
    &= 2 \sum_{k=1}^{\infty} k{}_{k}p_{x} - e_x - (e_x)^2
\end{aligned}
$$

### **Trapezoidal Rule**

Note that the two expectations are similar to one another:

* **Continuous Expectation** - Area under survival function
* **Discrete Expectation** - Right **Riemann Sum** of the area under the survival function

> A Right Riemann Sum is when the curve passes through the **top right** of the rectangles use to approximate it.

<!-- Obtained from Story of Mathematics -->
![Riemann Sum](Assets/1.%20Survival%20Models.md/Right%20Riemann%20Sum.png){.center}

Recall from Calculus that the area under a curve can be estimated through the **Trapezium Rule**, which states that the area is *approximately equal* to the sum of the area of discrete trapeziums formed under the curve.

$$
\begin{aligned}
    \int^b_a f(x)
    & \approx \sum \text{Area of Trapezium} \\
    & \approx \sum \frac{1}{2} h \left[f(a+kh) + f(a+(k+1)h) \right] \\
    & \approx \frac{h}{2}[f(a) + f(a+h)] + \frac{h}{2}[f(a+h) + f(a+2h)] + \dots + \frac{h}{2}[f(b-h) + f(b)] \\
    & \approx \frac{h}{2} f(a) + h[f(a+h) + f(a+2h) + \dots + f(b-h)] + \frac{h}{2} f(b) \\
    & \approx h[f(a+h) + f(a+2h) + \dots + f(b-h)] + \frac{h}{2} [f(a)+f(b)] \\
    & \approx h[f(a) + f(a+h) + \dots + f(b)] - \frac{h}{2} [f(a)+f(b)] \\
    & \approx h[f(a) + f(a+h) + \dots + f(b-h)] - \frac{h}{2} [f(a)-f(b)] \\
    & \approx h[f(a+h) + f(a+2h) + \dots + f(b)] + \frac{h}{2} [f(a)-f(b)]
\end{aligned}
$$

> The proof relies on the fact that other than $f(a)$ and $f(b)$, all other terms are repeated twice.

Note that the last four lines of the proof are all variations of the same thing:

1. Both $f(a)$ and $f(b)$ excluded from main expression
2. Both $f(a)$ and $f(b)$ included in main expression
3. Only $f(a)$ included in main expression; Main expression is a **Left Riemman Sum**
4. Only $f(b)$ included in main expression; Main expression is a **Right Riemman Sum**

<!-- Trapezium Rule -->
![Trapezium Rule](Assets/1.%20Survival%20Models.md/Trapezium%20Rule.png){.center}

Since the discrete expectation is a right riemann sum, the last expression of the trapezoidal rule should be used. This allows the continuous expectation to be expressed using the discrete expectation, assuming $h=1$:

$$
\begin{aligned}
    \mathring{e}_x
    &= \int^{\infty}_{0} S_x(t) \\
    & \approx h[f(a+h) + f(a+2h) + \dots + f(b)] + \frac{h}{2} [f(a)-f(b)] \\
    & \approx (1) [S_x(1) + S_x(2) + \dots + S_x(\infty)] + \frac{1}{2} [S_x(0)-S_x(\infty)] \\
    & \approx [S_x(1) + S_x(2) + \dots + S_x(\infty)] + \frac{1}{2} [1-0] \\
    & \approx e_x + \frac{1}{2}
\end{aligned}
$$

An alternative way to view the above is that the area of the trapezoid is the **sum of the riemann rectangles and a triangle**.

### **Euler Maclaurin Formula**

Note that the Trapezoidal Rule is *not perfect* - there is an **inherent error** in trying to approximate a curve using a line.

$$
\begin{aligned}
    \int^b_a f(x) & \approx \sum (\text{Area of Trapezium} + \text{Error})\\
\end{aligned}
$$

> The error can be positive or negative, depending on the shape of the curve in that interval.

<!-- Obtained from Wikipedia -->
![Trapezoidal Error](Assets/1.%20Survival%20Models.md/Trapezoidal%20Error.png){.center}

The error term is calculated by taking the difference between the integral and the trapezium, and is generalized using the taylor series. The final result is known as the **Euler Maclaurin Formula**:

$$
    \sum \text{Error} = \frac{h^2}{12} [f'(a)-f'(b)]
$$

> Given that a taylor series was used, the error can be expressed as the sum of many different terms, but **higher powers are ignored**.

Thus, the trapezoidal approximation for the expectation can be made more precise:

$$
\begin{aligned}
    \mathring{e}_x
    & \approx e_x + \frac{1}{2} + \frac{1^2}{12} [S'(0)-S'(\infty)] \\
    & \approx e_x + \frac{1}{2} + \frac{1}{12} [S'(0)]
\end{aligned}
$$

Note that the above two concepts are usually covered in the Life Annuities section in a more complicated scenario, known as the **Woolhouse Approximation**. Although the above will rarely be used in this manner, it provides a simple example to understand the key concepts behind it.

## **Parametric Survival Models**

Given the importance of $\mu_x$, several mathematical functions have been made to describe the force of mortality, known as a **Parametric Survival Model**.

### **De Moivre's Model**

### **Gompertz Model**

The most commonly used model is **Gompertz Model**, which suggests that mortality **increases exponentially with age**.

The is highly intuitive, as older people have a higher probability of death due to health issues related to age.

<!-- Obtained from Biodemography -->
![US Mortality](Assets/1.%20Survival%20Models.md/US%20Mortality.png)

It is interesting to note that the **ratio of death probabilities** year over year after the age of 30 is approximately constant - which means that the **death probability increases geometrically**.

Let $\lambda$ be the geometric mean of the death probabilities:

$$
\begin{aligned}
    q_{71} &= \lambda \cdot q_{70} \\
    \\
    q_{72}
    &= \lambda \cdot q_{71} \\
    &= \lambda^2 \cdot q_{70} \\
    \\
    \therefore q_{x+t} &= \lambda^t q_{x}
\end{aligned}
$$

<!-- Obtained from Biodemography -->
![Gompertz Parameter](Assets/1.%20Survival%20Models.md/Gompertz%20Parameter.png){.center}

Let $\lambda = e^b$. Thus, the model can be expressed continuously as the following:

$$
    \mu_{x+t} = Bc^{x+t}
$$

### **Makeham Gompertz Model**

Makeham added a **constant** $A$ into the Gompertz model, resulting in the **Makeham Gompertz Model**:

$$
    \mu_{x+t} = A + Bc^{x+t}
$$

$A$ represents the **age independent mortality** - dying from reasons unrelated to age, such as from accidents or natural catastrophes.

$$
\begin{aligned}
    S_x(t)
    &= - \int^{t}_{0} A + Bc^{x+t} \\
    &= \int^{t}_{0} -A - Bc^{x+t} \\
    &= \left[-At - \frac{B}{\ln c} c^{x+t} \right]^{t}_{0} \\
    &= \left[-At - \frac{B}{\ln c} c^{x+t} \right] - \left[-\frac{B}{\ln c} c^{x} \right] \\
    &= -At - \frac{B}{\ln c} c^{x+t} + \frac{B}{\ln c} c^{x} \\
    &= -At - \frac{B}{\ln c} c^x [c^t - 1]
\end{aligned}
$$